core/LoopV2.v
@@ -1,4 +1,4 @@
-Require Import Program List ZArith Arith Coq.Logic.Classical_Prop.
+(* Require Import Program List ZArith Arith Coq.Logic.Classical_Prop.
 
 Set Implicit Arguments.
 
@@ -530,3 +530,4 @@ max at level 60, body at level 60, right associativity) : monad_scope.
 
 Open Scope monad_scope.
 
+ *)
